Retrofitted regular executable semantics now extractable to CakeML

hol/retrofit_sem/p4_exec_wrapper_ffiLib.sig
@@ -1,0 +1,7 @@
+signature p4_exec_wrapper_ffiLib =
+sig
+  include Abbrev
+
+val translate_p4 : string -> term -> term -> term -> term -> bool -> bool -> unit
+
+end
