hol/retrofit_sem/p4_retrofit_auxLib.sig
@@ -1,0 +1,7 @@
+signature p4_retrofit_auxLib =
+sig
+  include Abbrev
+
+val get_id : string -> term
+
+end
