hol/retrofit_sem/p4_retrofit_auxLib.sml
@@ -1,0 +1,73 @@
+structure p4_retrofit_auxLib :> p4_retrofit_auxLib = struct
+
+open HolKernel boolLib liteLib simpLib Parse bossLib;
+
+open listSyntax bitstringSyntax numSyntax pairSyntax;
+
+open p4Theory;
+open p4Syntax;
+
+(* Note: This typically sets the word size that strings are serialized to in the CakeML-compilable
+ * semantics to either 32 or 64.
+ * Also works off the bat for 16 bits, but not 128.
+ * Could also be just strings. *)
+val identifier = “:string”;
+(* val identifier = “:word64”; *)
+(* val identifier = “:word32”; *)
+(* val identifier = “:word16”; *)
+
+(* This should hold all the named strings in core P4, and currently the additional ones for
+ * new architectures *)
+(* TODO: Move to top level? *)
+(* TODO: Can the parts of this belonging to the ext map be generated? *)
+val strings =
+ ["parseError", "err", "condition", "this", "headerLvalue", "targ1",
+  "bits", "data", "b", "b_temp", "standard_metadata", "parsedHdr", "hdr",
+  "meta", "check", "checksum", "algo", "size", "result", "index", "value",
+  "type", "ingress_port", "egress_spec", "egress_port", "instance_type",
+  "packet_length", "enq_timestamp", "enq_qdepth", "deq_timedelta",
+  "deq_qdepth", "ingress_global_timestamp", "egress_global_timestamp",
+  "mcast_grp", "egress_rid", "checksum_error", "parser_error", "priority",
+  "", "accept", "reject", "header", "packet_in", "packet_out",
+  "direct_counter", "register", "ipsec_crypt", "isValid", "setValid",
+  "setInvalid", "mark_to_drop", "verify", "verify_checksum",
+  "update_checksum", "assert", "assume", "extract", "lookahead", "advance",
+  "emit", "count", "read", "write", "decrypt_aes_ctr", "encrypt_aes_ctr",
+  "encrypt_null", "decrypt_null", "direct_meter", "action_selector",
+  "algorithm", "outputWidth", "packet_copy", "inCtrl", "packet",
+  "inputPort", "max_index", "CounterArray", "sparse", "increment", "add",
+  "headers"];
+
+(* As an SML association list *)
+val dict =
+ if wordsSyntax.is_word_type identifier
+ then
+  let
+   val width =
+    fcpSyntax.dest_int_numeric_type $ wordsSyntax.dest_word_type identifier;
+  in
+   rev $ foldl (fn (s, l) => ((s, wordsSyntax.mk_wordii (length l, width))::l)) [] strings
+  end
+ else if identifier = “:string”
+ then
+  foldr (fn (s, l) => ((s, stringSyntax.fromMLstring s)::l)) [] strings
+ else raise raise (mk_HOL_ERR "p4_retrofit_auxLib" "dict" ("identifier type not supported:"^(type_to_string identifier)));
+
+(* As a Redblackmap dict *)
+val cake_dict = Redblackmap.fromList String.compare dict;
+
+(* As a term *)
+val cake_dict_tm = mk_list (map (fn (a,b) => mk_pair (stringSyntax.fromMLstring a, b)) $ Redblackmap.listItems cake_dict, “:(string # ^identifier)”);
+
+fun get_id name =
+ let
+  val entry = Redblackmap.peek (cake_dict, name)
+ in
+  if isSome entry
+  then 
+   valOf entry
+  else raise (mk_HOL_ERR "p4_retrofit_auxLib" "get_id" ("key not found in cake_dict: "^name))
+ end
+;
+
+end
