hol/cake_sem/p4_cake_exec_semScript.sml
@@ -2175,9 +2175,4 @@ Definition p4_append_input_list'_def:
        ((ab_index, inputl++[h], outputl, ascope), gscope, afl, status)))
 End
 
-Definition p4_get_output_list_def:
- p4_get_output_list (((i, io_list, io_list', ascope), g_scope_list, arch_frame_list, status):'a astate') =
-  io_list'
-End
-
 val _ = export_theory ();
