hol/p4_coreScript.sml
@@ -2,7 +2,7 @@ open HolKernel boolLib Parse bossLib ottLib;
 
 val _ = new_theory "p4_core";
 
-open p4Theory p4_auxTheory;
+open p4Theory p4_auxTheory p4_exec_semTheory;
 
 (*****************)
 (* core ext type *)
@@ -16,6 +16,15 @@ open p4Theory p4_auxTheory;
 Datatype:
  core_v_ext =
   core_v_ext_packet (bool list)
+End
+
+(* Table type *)
+Datatype:
+tbl =
+   (* Any regular table *)
+   tbl_regular ((s list # num, (string # e_list)) alist)
+   (* A table with a custom implementation *)
+ | tbl_impl ((v list -> (string # e_list)))
 End
 
 (* NOTE: Definitions with _gen get specialised later by the different architectures *)
@@ -627,7 +636,7 @@ End
 Definition copyout_pbl_gen_def:
  copyout_pbl_gen xlist dlist g_scope_list v_map =
   let v_map_scope = v_map_to_scope v_map in
-   update_return_frame xlist dlist [v_map_scope] g_scope_list
+   update_return_frame_exec xlist dlist [v_map_scope] g_scope_list
 End
 
 (* A separate definition so that symbolic execution can choose to not evaluate it
@@ -705,6 +714,7 @@ End
 *)
 
 (* TODO: Are match_kinds needed at all in the dynamic semantics? *)
+(* OLD
 Definition FOLDL_MATCH_def:
  (FOLDL_MATCH e_l res [] = res) /\
  (FOLDL_MATCH e_l (res_act, res_prio_opt:num option) (((k,prio),v)::t) =
@@ -719,6 +729,23 @@ Definition FOLDL_MATCH_def:
     else FOLDL_MATCH e_l (res_act, res_prio_opt) t
    | NONE => FOLDL_MATCH e_l (v, SOME prio) t
   else FOLDL_MATCH e_l (res_act, res_prio_opt) t)
+End
+*)
+(* TODO: Updated for new tables *)
+Definition FOLDL_MATCH_def:
+ (FOLDL_MATCH w_l res [] = res) /\
+ (FOLDL_MATCH (w_l:v list) (res_act:string # e list, res_prio_opt:num option) (((s_l,prio),v)::t) =
+  if match_all_exec (ZIP(w_l, s_l))
+  then
+   (* TODO: Largest priority wins (like for P4Runtime API) is hard-coded *)
+   case res_prio_opt of
+   | SOME res_prio =>
+    if prio > res_prio
+    then
+     FOLDL_MATCH w_l (v, SOME prio) t
+    else FOLDL_MATCH w_l (res_act, res_prio_opt) t
+   | NONE => FOLDL_MATCH w_l (v, SOME prio) t
+  else FOLDL_MATCH w_l (res_act, res_prio_opt) t)
 End
 
 (*
@@ -738,6 +765,7 @@ End
 *)
 
 (* Alternative version, which uses smallest priority *)
+(* OLD
 Definition FOLDL_MATCH_alt_def:
  (FOLDL_MATCH_alt e_l res acc [] = res) /\
  (FOLDL_MATCH_alt e_l (res_act, res_prio_opt:num option) acc (((k,prio),v)::t) =
@@ -754,6 +782,25 @@ Definition FOLDL_MATCH_alt_def:
     else FOLDL_MATCH_alt e_l (res_act, res_prio_opt) (acc+1) t
    | NONE => FOLDL_MATCH_alt e_l (v, SOME prio) (acc+1) t
   else FOLDL_MATCH_alt e_l (res_act, res_prio_opt) (acc+1) t)
+End
+*)
+(* TODO: Updated for new tables *)
+Definition FOLDL_MATCH_alt_def:
+ (FOLDL_MATCH_alt w_l res acc [] = res) /\
+ (FOLDL_MATCH_alt w_l (res_act, res_prio_opt:num option) acc (((s_l,prio),v)::t) =
+  if match_all_exec (ZIP(w_l, s_l))
+  then
+   (* TODO: Smallest priority wins (like for TDI) is hard-coded,
+    *       other than priority zero. *)
+   case res_prio_opt of
+   | SOME res_prio =>
+    let prio' = if (prio = 0) then acc else prio in
+    if (prio' < res_prio)
+    then
+     FOLDL_MATCH_alt w_l (v, SOME prio') (acc+1) t
+    else FOLDL_MATCH_alt w_l (res_act, res_prio_opt) (acc+1) t
+   | NONE => FOLDL_MATCH_alt w_l (v, SOME prio) (acc+1) t
+  else FOLDL_MATCH_alt w_l (res_act, res_prio_opt) (acc+1) t)
 End
 
 val _ = export_theory ();
