hol/retrofit_sem/p4_exec_archScript.sml
@@ -1,0 +1,400 @@
+open HolKernel boolLib Parse bossLib;
+
+val _ = new_theory "p4_exec_arch";
+(* TODO: Remove? Almost nothing from here... *)
+
+open p4Syntax;
+open bitstringSyntax numSyntax pairSyntax;
+(*
+open p4Theory p4_auxTheory p4_cake_auxLib p4_cake_auxTheory p4_cake_exec_semTheory;
+
+open p4_retrofit_auxLib;
+
+open blahhhh;
+*)
+open p4Theory p4_auxTheory p4_retrofit_auxLib;
+open p4_coreTheory p4_v1modelTheory;
+
+(*********************)
+(* Core architecture *)
+
+(*
+Definition header_entries2v_def:
+ (header_entries2v (INL []) = SOME []) /\
+ (header_entries2v (INL (h::t)) =
+  case header_entries2v (INR h) of
+  | SOME bl =>
+  (case header_entries2v (INL t) of
+   | SOME bl2 => SOME (bl++bl2)
+   | NONE => NONE)
+  | NONE => NONE
+ ) /\
+ (header_entries2v (INR (x, v)) =
+  case v of
+  | (v_bit (bl, n)) => SOME bl
+  | (v_struct x_v_l) => header_entries2v (INL x_v_l)
+  | (v_header validity x_v_l) => header_entries2v (INL x_v_l)
+  | _ => NONE
+ )
+End
+*)
+(* Use regular ones
+(* TODO: Where's this used? *)
+Definition get_checksum_incr_def:
+ (get_checksum_incr (scope_list:scope_list) ext_data_name =
+   (case lookup_lval' scope_list ext_data_name of
+    | SOME (v_bit (bl, n)) =>
+     if n MOD 16 = 0 then (v2w16s''' bl) else NONE
+    | SOME (v_header vbit f_list) =>
+     (case header_entries2v (INL f_list) of
+      | SOME bl => v2w16s'' bl
+      | NONE => NONE)
+    | SOME (v_struct f_list) =>
+     (case header_entries2v (INL f_list) of
+      | SOME bl => v2w16s'' bl
+      | NONE => NONE)
+    | _ => NONE)
+ )
+End
+
+(** Some new architectural functions **)
+(*
+Definition v_map_to_scope_def:
+ (v_map_to_scope [] = []) /\
+ (v_map_to_scope (((k, v)::t)) =
+  ((varn_name k, (v:v, NONE:lval option))::v_map_to_scope t))
+End
+
+Definition scope_to_vmap_def:
+ (scope_to_vmap [] = SOME []) /\
+ (scope_to_vmap ((vn, (v:v, lval_opt:lval option))::t) =
+  case vn of
+   | (varn_name k) => oCONS ((k, v), scope_to_vmap t)
+   | _ => NONE)
+End
+
+Definition copyout_pbl_gen_def:
+ copyout_pbl_gen xlist dlist g_scope_list v_map =
+  let v_map_scope = v_map_to_scope v_map in
+   update_return_frame xlist dlist [v_map_scope] g_scope_list
+End
+*)
+
+(** Generic implementations **)
+Definition verify_gen_def:
+ (verify_gen ascope_update_v_map (ascope:'a, g_scope_list:g_scope_list, scope_list) =
+  case lookup_lval' scope_list (lval_varname (varn_name ^(get_id "condition"))) of
+  | SOME (v_bool T) =>
+   SOME (ascope, scope_list, status_returnv v_bot)
+  | SOME (v_bool F) =>
+   (case lookup_lval' scope_list (lval_varname (varn_name ^(get_id "err"))) of
+    | SOME (v_bit bitv) =>
+     SOME (ascope_update_v_map ascope ^(get_id "parseError") (v_bit bitv), scope_list, status_trans ^(get_id "reject"))
+    | _ => NONE)
+  | _ => NONE
+ )
+End
+
+Definition lookup_lval_header_def:
+ (lookup_lval_header ss header_lval =
+  case lookup_lval' ss header_lval of
+   | SOME (v_header valid_bit x_v_l) => SOME (valid_bit, x_v_l)
+   | _ => NONE
+ )
+End
+
+Definition size_in_bits_def:
+ (size_in_bits (v_bool b) = SOME 1) /\
+ (size_in_bits (v_bit (bl, n)) = SOME n) /\
+ (size_in_bits (v_header valid_bit []) = SOME 0) /\
+ (size_in_bits (v_struct []) = SOME 0) /\
+ (size_in_bits (v_header valid_bit (h::t)) =
+  case SND h of
+  | (v_bit (bl, num)) =>
+   (case size_in_bits (v_header valid_bit t) of
+    | SOME num' => SOME (num + num')
+    | NONE => NONE
+   )
+  | (v_bool _) =>
+   (case size_in_bits (v_header valid_bit t) of
+    | SOME num' => SOME (1 + num')
+    | NONE => NONE
+   )
+  | (v_struct flds) =>
+   (case size_in_bits (v_header valid_bit t) of
+    | SOME num' =>
+     (case size_in_bits (v_struct flds) of
+      | SOME num'' =>
+       SOME (num'' + num')
+      | NONE => NONE
+     )
+    | NONE => NONE
+   )
+  | _ => NONE
+ ) /\
+ (size_in_bits (v_struct (h::t)) =
+  case SND h of
+  | (v_bit (bl, num)) => 
+   (case size_in_bits (v_struct t) of
+    | SOME num' => SOME (num + num')
+    | NONE => NONE
+   )
+  | (v_bool _) =>
+   (case size_in_bits (v_struct t) of
+    | SOME num' => SOME (1 + num')
+    | NONE => NONE
+   )
+  | _ => NONE
+ ) /\
+ (size_in_bits _ = NONE)
+End
+
+Definition set_bool_def:
+ (set_bool [] = NONE) /\
+ (set_bool packet_in = SOME (v_bool (HD packet_in), TL packet_in))
+End
+Definition set_bit_def:
+ (set_bit n packet_in =
+  case oTAKE n packet_in of
+  | SOME res => SOME (v_bit (res, n), DROP n packet_in)
+  | NONE => NONE)
+End
+
+Definition set_fields_def:
+ (set_fields []     acc _ = SOME acc) /\
+ (set_fields (h::t) acc packet_in =
+  case h of
+  | (x:string, (v_bool b)) =>
+   (case set_bool packet_in of
+    | SOME (res, t') => set_fields t (acc++[(x, res)]) t'
+    | NONE => NONE)
+  | (x, (v_bit (bv, l))) =>
+   (case set_bit l packet_in of
+    | SOME (res, t') => set_fields t (acc++[(x, res)]) t'
+    | NONE => NONE)
+  | (x, (v_struct x_v_l)) =>
+   (case size_in_bits (v_struct x_v_l) of
+    | SOME n =>
+     (case oTAKE_DROP n packet_in of
+      | SOME (res, t') =>
+       (case set_fields x_v_l [] res of
+        | SOME acc' =>
+         set_fields t (acc++[(x, v_struct acc')]) t'
+        | NONE => NONE)
+      | NONE => NONE)
+    | NONE => NONE)
+  | _ => NONE)
+End
+
+Definition set_header_def:
+ (set_header x_v_l packet_in =
+  case set_fields x_v_l [] packet_in of
+  | SOME x_v_l' => SOME (v_header T x_v_l')
+  | NONE => NONE)
+End
+
+Definition set_struct_def:
+ (set_struct x_v_l packet_in =
+  case set_fields x_v_l [] packet_in of
+  | SOME x_v_l' => SOME (v_struct x_v_l')
+  | NONE => NONE)
+End
+
+Definition set_v_def:
+ (set_v (v_bit (bitv, n)) packet_in =
+  case set_bit n packet_in of
+  | SOME (res, t') => SOME res
+  | NONE => NONE) /\
+ (set_v (v_bool b)        packet_in =
+  case set_bool packet_in of
+  | SOME (res, t') => SOME res
+  | NONE => NONE) /\
+ (set_v (v_struct x_v_l) packet_in = (set_struct x_v_l packet_in)) /\
+ (set_v (v_header validity x_v_l) packet_in = (set_header x_v_l packet_in)) /\
+ (set_v _ packet_in = NONE)
+End
+
+
+
+Definition packet_in_extract_gen_def:
+ (packet_in_extract_gen ascope_lookup ascope_update ascope_update_v_map (ascope:'a, g_scope_list:g_scope_list, scope_list) =
+  case lookup_lval' scope_list (lval_varname (varn_name ^(get_id "this"))) of
+  | SOME (v_ext_ref i) =>
+   (case lookup_lval_header scope_list (lval_varname (varn_name ^(get_id "headerLvalue"))) of
+    | SOME (valid_bit, x_v_l) =>
+     (case lookup_ascope_gen ascope_lookup ascope i of
+      | SOME ((INL (core_v_ext_packet packet_in_bl)):(core_v_ext, 'b) sum) =>
+       (case size_in_bits (v_header valid_bit x_v_l) of
+        | SOME sz =>
+           if sz <= LENGTH packet_in_bl
+           then
+             (case set_header x_v_l packet_in_bl of
+              | SOME header =>
+               (case assign' scope_list header (lval_varname (varn_name ^(get_id "headerLvalue"))) of
+                | SOME scope_list' =>
+                 SOME (update_ascope_gen ascope_update ascope i ((INL (core_v_ext_packet (DROP sz packet_in_bl))):(core_v_ext, 'b) sum), scope_list', status_returnv v_bot)
+                | NONE => NONE)
+              | NONE => NONE)
+           else
+            (* NOTE: Specific serialisation of errors is assumed here - "PacketTooShort" -> 1 *)
+            SOME (ascope_update_v_map (update_ascope_gen ascope_update ascope i ((INL (core_v_ext_packet [])):(core_v_ext, 'b) sum)) ^(get_id "parseError") (v_bit (fixwidth 32 (n2v 1), 32)), scope_list, status_trans ^(get_id "reject"))
+        | NONE => NONE)
+       | _ => NONE)
+    | NONE => NONE)
+  | _ => NONE
+ )
+End
+
+Definition packet_in_lookahead_gen_def:
+ (packet_in_lookahead_gen ascope_lookup ascope_update_v_map (ascope:'a, g_scope_list:g_scope_list, scope_list) =
+  case lookup_lval' scope_list (lval_varname (varn_name ^(get_id "this"))) of
+  | SOME (v_ext_ref i) =>
+   (case lookup_lval' scope_list (lval_varname (varn_name ^(get_id "targ1"))) of
+    | SOME dummy_v =>
+     (case lookup_ascope_gen ascope_lookup ascope i of
+      | SOME ((INL (core_v_ext_packet packet_in_bl)):(core_v_ext, 'b) sum) =>
+       (case size_in_bits dummy_v of
+        | SOME sz =>
+          if sz <= LENGTH packet_in_bl
+          then
+             (case set_v dummy_v packet_in_bl of
+              | SOME v =>
+               SOME (ascope, scope_list, status_returnv v)
+              | NONE => NONE)
+          else
+           (* NOTE: Specific serialisation of errors is assumed here - "PacketTooShort" -> 1 *)
+           SOME (ascope_update_v_map ascope ^(get_id "parseError") (v_bit (fixwidth 32 (n2v 1), 32)), scope_list, status_trans ^(get_id "reject"))
+        | NONE => NONE)
+       | _ => NONE)
+    | NONE => NONE)
+  | _ => NONE
+ )
+End
+
+Definition lookup_lval_bit32_def:
+ (lookup_lval_bit32 ss bit32_lval =
+  case lookup_lval' ss bit32_lval of
+   | SOME (v_bit (bitv, 32)) => SOME (v2n bitv)
+   | _ => NONE
+ )
+End
+Definition packet_in_advance_gen_def:
+ (packet_in_advance_gen ascope_lookup ascope_update ascope_update_v_map (ascope:'a, g_scope_list:g_scope_list, scope_list) =
+  case lookup_lval' scope_list (lval_varname (varn_name ^(get_id "this"))) of
+  | SOME (v_ext_ref i) =>
+   (case lookup_lval_bit32 scope_list (lval_varname (varn_name ^(get_id "bits"))) of
+    | SOME n_bits =>
+     (case lookup_ascope_gen ascope_lookup ascope i of
+      | SOME ((INL (core_v_ext_packet packet_in_bl)):(core_v_ext, 'b) sum) =>
+        if n_bits <= LENGTH packet_in_bl
+        then
+         SOME (update_ascope_gen ascope_update ascope i ((INL (core_v_ext_packet (DROP n_bits packet_in_bl))):(core_v_ext, 'b) sum), scope_list, status_returnv v_bot)
+        else
+         (* NOTE: Serialisation of errors is assumed here - "PacketTooShort" -> 1 *)
+         SOME (ascope_update_v_map ascope ^(get_id "parseError") (v_bit (fixwidth 32 (n2v 1), 32)), scope_list, status_trans ^(get_id "reject"))
+       | _ => NONE)
+    | NONE => NONE)
+  | _ => NONE
+ )
+End
+
+Definition flatten_v_l_def:
+ (flatten_v_l [] = SOME []) /\
+ (flatten_v_l (h::t) =
+  case h of
+  | v_struct [] =>
+   (case flatten_v_l t of
+    | SOME l => SOME l
+    | NONE => NONE)
+  | v_struct (h'::t') =>
+   (case flatten_v_l [SND h'] of
+    | SOME l =>
+     (case flatten_v_l ((v_struct t')::t) of
+      | SOME l' => SOME (l++l')
+      | NONE => NONE)
+    | NONE => NONE)
+  | v_header validity [] =>
+   (case flatten_v_l t of
+    | SOME l => SOME l
+    | NONE => NONE)
+  | v_header validity (h'::t') =>
+   (case flatten_v_l [SND h'] of
+    | SOME l =>
+     (case flatten_v_l ((v_struct t')::t) of
+      | SOME l' => SOME (l++l')
+      | NONE => NONE)
+    | NONE => NONE)
+  | v_bit (bl, n) =>
+   (case flatten_v_l t of
+    | SOME l => SOME (bl++l)
+    | NONE => NONE)
+  | v_bool b =>
+   (case flatten_v_l t of
+    | SOME l => SOME (b::l)
+    | NONE => NONE)
+  | _ => NONE
+ )
+End
+Definition packet_out_emit_gen_def:
+ (packet_out_emit_gen (ascope_lookup:'a -> num -> (core_v_ext + 'b) option) ascope_update (ascope:'a, g_scope_list:g_scope_list, scope_list) =
+  case lookup_lval' scope_list (lval_varname (varn_name ^(get_id "this"))) of
+  | SOME (v_ext_ref i) =>
+   (case lookup_ascope_gen ascope_lookup ascope i of
+    | SOME (INL (core_v_ext_packet packet_out_bl)) =>
+     (case lookup_lval' scope_list (lval_varname (varn_name ^(get_id "data"))) of
+      | SOME (v_header F x_v_l) => SOME (ascope, scope_list, status_returnv v_bot)
+      | SOME (v_header T x_v_l) =>
+       (case flatten_v_l (MAP SND x_v_l) of
+        | SOME bl =>
+           SOME (update_ascope_gen ascope_update ascope i ((INL (core_v_ext_packet (packet_out_bl++bl))):(core_v_ext, 'b) sum), scope_list, status_returnv v_bot)
+        | NONE => NONE)
+      | SOME (v_struct x_v_l) =>
+       (case flatten_v_l (MAP SND x_v_l) of
+        | SOME bl =>
+           SOME (update_ascope_gen ascope_update ascope i ((INL (core_v_ext_packet (packet_out_bl++bl))):(core_v_ext, 'b) sum), scope_list, status_returnv v_bot)
+        | NONE => NONE)
+      | SOME _ => NONE
+      | NONE => NONE)
+    | _ => NONE)
+  | _ => NONE
+ )
+End
+
+
+(** Implementations **)
+
+Definition header_is_valid_def:
+ (header_is_valid (ascope:'a, g_scope_list:g_scope_list, scope_list) =
+  case lookup_lval' scope_list (lval_varname (varn_name ^(get_id "this"))) of
+  | SOME (v_header valid_bit x_v_l) =>
+   SOME (ascope, scope_list, status_returnv (v_bool valid_bit))
+  | _ => NONE
+ )
+End
+
+
+Definition header_set_valid_def:
+ (header_set_valid (ascope:'a, g_scope_list:g_scope_list, scope_list) =
+  case lookup_lval' scope_list (lval_varname (varn_name ^(get_id "this"))) of
+  | SOME (v_header valid_bit x_v_l) =>
+   (case assign' scope_list (v_header T x_v_l) (lval_varname (varn_name ^(get_id "this"))) of
+    | SOME scope_list' =>
+     SOME (ascope, scope_list', status_returnv v_bot)
+    | NONE => NONE)
+  | _ => NONE
+ )
+End
+
+Definition header_set_invalid_def:
+ (header_set_invalid (ascope:'a, g_scope_list:g_scope_list, scope_list) =
+  case lookup_lval' scope_list (lval_varname (varn_name ^(get_id "this"))) of
+  | SOME (v_header valid_bit x_v_l) =>
+   (case assign' scope_list (v_header F x_v_l) (lval_varname (varn_name ^(get_id "this"))) of
+    | SOME scope_list' =>             
+     SOME (ascope, scope_list', status_returnv v_bot)
+    | NONE => NONE)
+  | _ => NONE
+ )
+End
+*)
+val _ = export_theory ();
