hol/retrofit_sem/p4_exec_arch_v1modelProgScript.sml
@@ -1,0 +1,112 @@
+open HolKernel boolLib Parse bossLib;
+
+val _ = new_theory "p4_exec_arch_v1modelProg";
+
+open p4Theory p4_auxTheory p4_coreTheory p4_v1modelTheory;
+open p4_exec_archTheory p4_exec_arch_v1modelTheory;
+open p4_exec_semTheory;
+open p4_exec_semProgTheory;
+
+(* CakeML: *)
+open preamble ml_translatorLib ml_progLib basisProgTheory;
+
+intLib.deprecate_int();
+val _ = (max_print_depth := 100);
+
+val _ = translation_extends "p4_exec_semProg";
+
+val _ = ml_prog_update (open_module "p4_exec_arch_v1modelProg");
+
+(** V1Model arch implementation **)
+
+(* Architectural functions: *)
+
+val _ = translate v_map_to_scope_def;
+val _ = translate oCONS_def;
+val _ = translate scope_to_vmap_def;
+val _ = translate v1model_ascope_update_def;
+
+val _ = translate v1model_postparser_def;
+val _ = translate v1model_preingress_def;
+
+val _ = translate v1model_input_f_def;
+
+val _ = translate v1model_is_drop_port_def;
+val _ = translate v1model_lookup_obj_def;
+val _ = translate v1model_output_f_def;
+
+val _ = translate v1model_reduce_nonout_def;
+val _ = translate v1model_copyin_pbl_def;
+
+val _ = translate copyout_pbl_gen_def;
+val _ = translate v1model_copyout_pbl_def;
+
+val _ = translate FOLDL_MATCH_alt_def;
+val _ = translate FOLDL_MATCH_def;
+val _ = translate listTheory.LIST_TO_SET_DEF;
+val _ = translate boolTheory.IN_DEF;
+val _ = translate v1model_apply_table_f''_def;
+
+(* Extern implementations: *)
+
+val _ = translate v1model_mark_to_drop_def;
+
+val _ = translate v1model_ascope_update_v_map_def;
+val _ = translate verify_gen_def;
+val _ = translate v1model_verify_def;
+
+val _ = translate v1model_assert_def;
+
+val _ = translate v1model_assume_def;
+
+val _ = translate v1model_verify_checksum_def;
+
+val _ = translate v1model_update_checksum_def;
+
+val _ = translate lookup_lval_header_def;
+val _ = translate lookup_ascope_gen_def;
+val _ = translate size_in_bits_def;
+val _ = translate set_bool_def;
+val _ = translate set_bit_def;
+val _ = translate set_fields_def;
+val _ = translate set_header_def;
+val _ = translate update_ascope_gen_def;
+val _ = translate packet_in_extract_gen_def;
+val _ = translate v1model_ascope_lookup_def;
+val _ = translate v1model_packet_in_extract_def;
+
+val _ = translate set_struct_def;
+val _ = translate set_v_def;
+val _ = translate packet_in_lookahead_gen_def;
+val _ = translate v1model_packet_in_lookahead_def;
+
+val _ = translate lookup_lval_bit32_def;
+val _ = translate packet_in_advance_gen_def;
+val _ = translate v1model_packet_in_advance_def;
+
+val _ = translate flatten_v_l_def;
+val _ = translate packet_out_emit_gen_def;
+val _ = translate v1model_packet_out_emit_def;
+
+val _ = translate v1model_direct_counter_construct_def;
+val _ = translate v1model_direct_counter_count_def;
+
+val _ = translate v1model_direct_meter_construct_def;
+
+val _ = translate v1model_action_selector_construct_def;
+
+(* TODO: The below is defined in terms of functions that uses ARB... *)
+(*
+val _ = translate v1model_register_construct_inner_def;
+val _ = translate register_construct_def;
+
+val _ = translate v1model_register_read_inner_def;
+val _ = translate register_read'_def;
+
+val _ = translate v1model_register_write_inner_def;
+val _ = translate register_write'_def;
+*)
+
+val _ = ml_prog_update (close_module NONE);
+
+val _ = export_theory ();
