hol/retrofit_sem/p4_exec_arch_v1modelScript.sml
@@ -1,0 +1,131 @@
+open HolKernel boolLib Parse bossLib;
+
+val _ = new_theory "p4_exec_arch_v1model";
+
+open p4Syntax;
+open bitstringSyntax numSyntax pairSyntax;
+open p4Theory p4_auxTheory p4_retrofit_auxLib p4_exec_semTheory p4_exec_archTheory;
+open p4_coreTheory p4_v1modelTheory;
+
+val CONTROL_PLANE_API = 0;
+
+(*
+(* TODO: Retrofitted this *)
+Definition v1model_input_f_def:
+ (v1model_input_f (tau1_uninit_v,tau2_uninit_v) (io_list:in_out_list, (counter, ext_obj_map, v_map, ctrl):v1model_ascope) =
+  case io_list of
+  | [] => NONE
+  | ((byte_list,p)::t) =>
+   (* TODO: Implement persistence between packets when you fully model persistent extern objects *)
+   let ext_obj_map' = AUPDATE_LIST [] [(0, INL (core_v_ext_packet byte_list));
+                                       (1, INL (core_v_ext_packet []))] in
+   let counter' = 2 in
+   (* TODO: Currently, no garbage collection in v_map is needed *)
+   let v_map' = AUPDATE_LIST v_map [(^(get_id "b"), v_ext_ref 0);
+                                    (^(get_id "b_temp"), v_ext_ref 1);
+                                    (^(get_id "standard_metadata"), v_struct (p4$AUPDATE (^v1model_standard_metadata_zeroed) (^(get_id "ingress_port"), (v_bit (fixwidth 9 $ n2v p, 9) ) )));
+                                    (^(get_id "parsedHdr"), tau1_uninit_v);
+                                    (^(get_id "hdr"), tau1_uninit_v);
+                                    (^(get_id "meta"), tau2_uninit_v);
+                                    (^(get_id "checksum_error"), v_bit ([F], 1))] in
+    SOME (t, (counter', ext_obj_map', v_map', ctrl):v1model_ascope))
+End
+*)
+
+(* TODO: Regular version hacked to use init_out_v_cake
+(* TODO: Uninit? *)
+Definition v1model_reduce_nonout_def:
+ (v1model_reduce_nonout ([], elist:e list, v_map) =
+  SOME []
+ ) /\
+ (v1model_reduce_nonout (d::dlist, e::elist, v_map) =
+  if is_d_out d
+  then oCONS (e, v1model_reduce_nonout (dlist, elist, v_map))
+  else
+   (case e of
+    | (e_var (varn_name x)) =>
+     (case ALOOKUP v_map x of
+      | SOME v =>
+       if is_d_in d
+       then oCONS (e_v v, v1model_reduce_nonout (dlist, elist, v_map))
+       else oCONS (e_v (init_out_v_cake v), v1model_reduce_nonout (dlist, elist, v_map))       
+      | _ => NONE)
+    | _ => NONE)) /\
+ (v1model_reduce_nonout (_, _, v_map) = NONE)
+End
+*)
+
+(* TODO: Regular version hacked to use copyin_exec
+(* Uses the above and copyin *)
+Definition v1model_copyin_pbl_def:
+ v1model_copyin_pbl (xlist, dlist, elist, (counter, ext_obj_map, v_map, ctrl):v1model_ascope) =
+  case v1model_reduce_nonout (dlist, elist, v_map) of
+  | SOME elist' =>
+   (case copyin_exec xlist dlist elist' [v_map_to_scope v_map] [ [] ] of
+    | SOME scope =>
+     SOME scope
+    | NONE => NONE)
+  | NONE => NONE
+End
+*)
+(* TODO: Just forget about registers, for now...
+Definition register_construct_def:
+ (register_construct ((counter, ext_obj_map, v_map, ctrl):v1model_ascope, g_scope_list:g_scope_list, scope_list) =
+  case lookup_lval_exec scope_list (lval_varname (varn_name ^(get_id "size"))) of
+  | SOME (v_bit (bl, n)) =>
+   (case lookup_lval_exec scope_list (lval_varname (varn_name ^(get_id "targ1"))) of
+    | SOME (v_bit (bl', n')) =>
+     let ext_obj_map' = AUPDATE ext_obj_map (counter, INR (v1model_v_ext_register (v1model_register_construct_inner bl n'))) in
+     (case assign_exec scope_list (v_ext_ref counter) (lval_varname (varn_name ^(get_id "this"))) of
+      | SOME scope_list' =>
+       SOME ((counter + 1, ext_obj_map', v_map, ctrl), scope_list', status_returnv v_bot)
+      | NONE => NONE)
+    | _ => NONE)
+  | _ => NONE
+ )
+End
+
+Definition register_read_def:
+ (register_read ((counter, ext_obj_map, v_map, ctrl):v1model_ascope, g_scope_list:g_scope_list, scope_list) =
+  case lookup_lval_exec scope_list (lval_varname (varn_name ^(get_id "index"))) of
+  | SOME (v_bit (bl, n)) =>
+   (case lookup_lval_exec scope_list (lval_varname (varn_name ^(get_id "this"))) of
+    | SOME (v_ext_ref i) =>
+     (case ALOOKUP ext_obj_map i of
+      | SOME (INR (v1model_v_ext_register array)) =>
+       (* TODO: HACK, looking up the result variable to get the result width. *)
+       (case lookup_lval_exec scope_list (lval_varname (varn_name ^(get_id "result"))) of
+        | SOME (v_bit (bl'', n'')) =>      
+         let (bl', n') = v1model_register_read_inner n'' bl array in
+           (case assign_exec scope_list (v_bit (bl', n')) (lval_varname (varn_name ^(get_id "result"))) of
+            | SOME scope_list' =>
+             SOME ((counter, ext_obj_map, v_map, ctrl), scope_list', status_returnv v_bot)
+            | NONE => NONE)
+        | _ => NONE)
+      | _ => NONE)
+    | _ => NONE)
+  | _ => NONE
+ )
+End
+
+Definition register_write_def:
+ (register_write ((counter, ext_obj_map, v_map, ctrl):v1model_ascope, g_scope_list:g_scope_list, scope_list) =
+  case lookup_lval_exec scope_list (lval_varname (varn_name ^(get_id "index"))) of
+  | SOME (v_bit (bl, n)) =>
+   (case lookup_lval_exec scope_list (lval_varname (varn_name ^(get_id "value"))) of
+    | SOME (v_bit (bl', n')) =>
+     (case lookup_lval_exec scope_list (lval_varname (varn_name ^(get_id "this"))) of
+      | SOME (v_ext_ref i) =>
+       (case ALOOKUP ext_obj_map i of
+        | SOME (INR (v1model_v_ext_register array)) =>
+         let array' = v1model_register_write_inner (bl', n') bl array in
+         let ext_obj_map' = AUPDATE ext_obj_map (i, INR (v1model_v_ext_register array')) in
+          SOME ((counter, ext_obj_map', v_map, ctrl), scope_list, status_returnv v_bot)
+        | _ => NONE)
+      | _ => NONE)
+    | _ => NONE)
+  | _ => NONE
+ )
+End
+*)
+val _ = export_theory ();
