hol/retrofit_sem/p4_exec_semProgScript.sml
@@ -1,0 +1,452 @@
+open HolKernel boolLib Parse bossLib;
+
+val _ = new_theory "p4_exec_semProg";
+
+open p4Theory p4_auxTheory p4_coreTheory p4_v1modelTheory
+     p4_exec_semTheory;
+open p4_exec_archTheory;
+
+(* CakeML: *)
+open preamble ml_translatorLib ml_progLib basisProgTheory;
+
+intLib.deprecate_int();
+val _ = (max_print_depth := 100);
+
+val _ = translation_extends "basisProg";
+
+val _ = ml_prog_update (open_module "p4_exec_semProg");
+
+(************************)
+(* Expression semantics *)
+
+(* Variable look-up *)
+val _ = translate INDEX_FIND_def;
+val _ = translate find_topmost_map_def;
+val _ = translate topmost_map_def;
+val _ = translate lookup_map_def;
+val _ = translate lookup_vexp2_def;
+
+(* Struct/header field access *)
+val _ = translate is_v_def;
+val _ = translate e_exec_acc_def;
+
+(* Unary arithmetic *)
+val _ = translate bitv_1comp_def;
+val _ = translate numposrepTheory.l2n_def;
+val _ = translate bitstringTheory.bitify_def;
+val _ = translate bitstringTheory.v2n_def;
+Theorem l2n_side_thm:
+!n l. l2n_side n l <=> (l <> [] ==> n <> 0)
+Proof
+strip_tac \\
+Induct \\ (
+ rpt strip_tac \\
+ ONCE_REWRITE_TAC[theorem "l2n_side_def"] \\
+ gs[]
+) \\
+Cases_on ‘l’ \\ (
+ gs[]
+)
+QED
+val _ = update_precondition l2n_side_thm;
+Theorem v2n_side:
+!v1. v2n_side v1
+Proof
+gs[definition "v2n_side_def", l2n_side_thm, bitstringTheory.bitify_def]
+QED
+val _ = update_precondition v2n_side;
+val _ = translate bitstringTheory.zero_extend_def;
+val _ = translate listTheory.DROP_def;
+val _ = translate bitstringTheory.boolify_def;
+val _ = translate numposrepTheory.n2l_def;
+val _ = translate bitstringTheory.n2v_def;
+Theorem n2l_side_thm:
+!n m. n2l_side n m <=> n <> 0
+Proof
+strip_tac \\
+completeInduct_on ‘m’ \\
+rpt strip_tac \\
+ONCE_REWRITE_TAC[theorem "n2l_side_def"] \\
+gs[]
+QED
+val _ = update_precondition n2l_side_thm;
+Theorem n2v_side:
+!v. n2v_side v
+Proof
+gs[definition "n2v_side_def", n2l_side_thm]
+QED
+val _ = update_precondition n2v_side;
+val _ = translate bitstringTheory.fixwidth_def;
+val _ = translate bitv_2comp_def;
+Theorem bitv_2comp_side:
+!v. bitv_2comp_side v
+Proof
+gs[definition "bitv_2comp_side_def", arithmeticTheory.LT_IMP_LE, bitstringTheory.v2n_lt]
+QED
+val _ = update_precondition bitv_2comp_side;
+val _ = translate unop_exec_def;
+val _ = translate e_exec_unop_def;
+
+(* Cast *)
+val _ = translate bool_cast_def;
+val _ = translate bitv_cast_def;
+val _ = translate oHD_def;
+val _ = translate to_bool_cast_exec_def;
+val _ = translate cast_exec_def;
+val _ = translate e_exec_cast_def;
+
+(* Binary arithmetic *)
+val _ = translate is_short_circuitable_def;
+val _ = translate e_exec_short_circuit_def;
+
+val _ = translate bitv_mul_def;
+val _ = translate bitv_div_def;
+val _ = translate bitv_mod_def;
+val _ = translate bitv_add_def;
+val _ = translate bitv_sub_def;
+val _ = translate band'_def;
+val _ = translate bitv_and_def;
+val _ = translate bor'_def;
+val _ = translate bitv_or_def;
+val _ = translate bitstringTheory.bitwise_def;
+val _ = translate bitstringTheory.bxor_def;
+val _ = translate bitv_xor_def;
+val _ = translate rich_listTheory.REPLICATE;
+val _ = translate bitv_saturate_add_def;
+val _ = translate bitv_saturate_sub_def;
+val _ = translate bitv_lsl_bv_def;
+val _ = translate TAKE_def;
+val _ = translate bitv_lsr_bv_def;
+val _ = translate get_bitv_binop'_def;
+val _ = translate bitv_binop'_def;
+
+val _ = translate bitv_bl_binop_def;
+val _ = translate bitstringTheory.shiftl_def;
+
+val _ = translate bitv_ls_def;
+val _ = translate bitv_hs_def;
+val _ = translate bitv_lo_def;
+val _ = translate bitv_hi_def;
+val _ = translate rich_listTheory.AND_EL_DEF;
+val _ = translate bit_eq_def;
+val _ = translate bitv_eq_def;
+val _ = translate bitv_neq_def;
+val _ = translate get_bitv_binpred'_def;
+val _ = translate bitv_binpred'_def;
+
+val _ = translate binop_exec_def;
+val _ = translate e_exec_binop_def;
+
+(* Concatenation *)
+val _ = translate bitv_concat_def;
+val _ = translate e_exec_concat_def;
+val _ = translate is_v_bit_def;
+
+(* Slicing *)
+val _ = translate rich_listTheory.SEG;
+Theorem seg_side_thm:
+!len start l. seg_side len start l <=> (len <> 0 ==> (start + len <= LENGTH l))
+Proof
+strip_tac \\
+completeInduct_on ‘len’ \\
+completeInduct_on ‘start’ \\
+rpt strip_tac \\
+ONCE_REWRITE_TAC[theorem "seg_side_def"] \\
+gs[] \\
+eq_tac >- (
+ rpt strip_tac >- (
+  res_tac \\
+  gs[]
+ ) \\
+ gs[] \\
+ qpat_x_assum ‘!m. m < SUC x4 ==>
+               !l'. seg_side (SUC x3) m l' <=> m + SUC x3 <= LENGTH l'’
+              (fn thm => ASSUME_TAC $ Q.SPEC ‘x4’ thm) \\
+ gs[arithmeticTheory.SUC_ONE_ADD]
+) \\
+rpt strip_tac \\ (
+ gs[]
+) >- (
+ Cases_on ‘len’ \\ Cases_on ‘start’ \\ (
+  gs[]
+ ) >- (
+  Cases_on ‘l’ \\ (
+   gs[]
+  )
+ ) \\
+ Cases_on ‘l’ \\ (
+  gs[]
+ )
+) \\
+qpat_x_assum ‘!m. m < SUC x10 ==>
+              !l'. seg_side (SUC x13) m l' <=> m + SUC x13 <= LENGTH l'’
+             (fn thm => ASSUME_TAC $ Q.SPEC ‘x10’ thm) \\
+gvs[] \\
+gs[arithmeticTheory.SUC_ONE_ADD]
+QED
+val _ = update_precondition seg_side_thm;
+val _ = translate bitv_bitslice_def;
+val _ = translate slice'_def;
+Theorem slice'_side:
+!v1 v2 v3. slice'_side v1 v2 v3
+Proof
+simp[Once $ definition "slice'_side_def"] \\
+simp[Once $ definition "bitv_bitslice_side_def"]
+QED
+val _ = update_precondition slice'_side;
+val _ = translate e_exec_slice_def;
+
+(* Function call *)
+val _ = translate lookup_funn_sig_body_def;
+
+val _ = translate is_d_out_def;
+
+val _ = translate get_lval_of_e_def;
+
+val _ = translate is_e_lval_def;
+val _ = translate is_const_def;
+val _ = translate is_arg_red_def;
+val _ = translate find_unred_arg_def;
+val _ = translate unred_arg_index_def;
+
+val _ = translate is_d_in_def;
+val _ = translate bitstringTheory.extend_def;
+(* TODO: Fix the uninit hack
+val _ = translate uninit_bit_def;
+val _ = translate uninit_string_def;
+val _ = translate init_out_v_gen_def;
+*)
+val _ = translate init_out_v_cake_def;
+
+val _ = translate slice_lval'_def;
+val _ = translate acc_f_def;
+val _ = translate lookup_v_def;
+val _ = translate lookup_lval'_def;
+
+val _ = translate v_of_e_def;
+val _ = translate one_arg_val_for_newscope_exec_def;
+
+val _ = translate AFUPDKEY_def;
+val _ = translate AUPDATE_def;
+val _ = translate update_arg_for_newscope_exec_def;
+val _ = translate listTheory.FOLDL;
+val _ = translate all_arg_update_for_newscope_exec_def;
+val _ = translate copyin_exec_def;
+
+val _ = translate oEL_def;
+
+(* Select *)
+
+val _ = translate p4_match_range_exec_def;
+val _ = translate p4_match_mask_exec_def;
+val _ = translate match_exec_def;
+val _ = translate match_all_exec_def;
+val _ = translate pre_match_check_def;
+val _ = translate e_exec_select_def;
+
+(* Struct *)
+
+val _ = translate unred_mem_def;
+val _ = translate unred_mem_index_def;
+
+val _ = translate get_v_def;
+val _ = translate vl_of_el_exec_def;
+
+(* The whole expression-level semantics: *)
+val _ = translate e_exec_def;
+(*
+(* TODO: This should be inherited from uninit_zero on the
+ * level above *)
+Theorem e_exec_side:
+!a b c d e. e_exec_side a b c d e
+Proof
+cheat
+QED
+val _ = update_precondition e_exec_side;
+*)
+
+(*************************)
+(** Statement semantics **)
+
+val _ = translate get_e_ctx_def;
+
+(* Assignment *)
+val _ = translate separate_exec_def;
+
+val _ = translate lookup_out_def;
+val _ = translate replace_bits_def;
+val _ = translate assign_to_slice'_def;
+val _ = translate listTheory.INDEX_OF_def;
+val _ = translate assign'_def;
+val _ = translate stmt_exec_ass_def;
+
+(* Conditional *)
+val _ = translate is_v_bool_def;
+val _ = translate stmt_exec_cond_def;
+
+(* Block *)
+(* TODO: Fix this hack *)
+val _ = translate init_v_from_tau_cake_def;
+val _ = translate declare_list_in_fresh_scope_exec'_def;
+(*
+val _ = translate uninit_num_def;
+val _ = translate arb_from_tau_gen_def;
+val _ = translate declare_list_in_fresh_scope_exec_def;
+(* TODO: This should be inherited from uninit_zero on the
+ * level above *)
+Theorem declare_list_in_fresh_scope_exec_side:
+!a b. declare_list_in_fresh_scope_exec_side a b
+Proof
+cheat
+QED
+val _ = update_precondition declare_list_in_fresh_scope_exec_side;
+*)
+
+(* Return *)
+
+(* Sequence *)
+val _ = translate is_empty_def;
+
+(* Transition *)
+val _ = translate is_v_str_def;
+val _ = translate stmt_exec_trans_def;
+
+(* Apply *)
+val _ = translate index_not_const_def;
+
+val _ = translate is_consts_exec_def;
+
+(* Extern *)
+val _ = translate lookup_ext_fun_def;
+
+
+(* ??? Why? *)
+val _ = translate oDROP_def;
+val _ = translate oTAKE_def;
+
+(* The whole stmt semantics *)
+val _ = translate stmt_exec_stack_finish_def;
+val _ = translate stmt_exec_seq_finish_def;
+(* ~14 mins of nothing, then
+
+<<HOL warning: ThmSetData.revise_data: 
+  Theorems in set "compute":
+    ADD<scratch$generated_definition_def>
+  invalidated by DelConstant(scratch$generated_definition)>>
+  
+then 3 minutes of silence, then
+
+     Translating stmt_exec
+
+then around a minute before finishing.
+
+Total time: 16m52s
+*)
+val _ = translate stmt_exec_def;
+
+
+(*********************)
+(** Frame semantics **)
+
+val _ = translate scopes_to_pass_exec_def;
+val _ = translate scopes_to_retrieve_exec_def;
+val _ = translate map_to_pass_def;
+val _ = translate tbl_to_pass_def;
+val _ = translate is_d_none_in_def;
+
+val _ = translate update_return_frame_exec_def;
+val _ = translate copyout_exec_def;
+
+(* 29s - uninit precondition (cheated on level below) *)
+val _ = translate frames_exec_def;
+
+
+(********************)
+(** Arch semantics **)
+val _ = translate lookup_block_body_def;
+val _ = translate oLASTN_def;
+
+(* TODO: Fix this hack *)
+val _ = translate init_v_from_tau_cake_def;
+val _ = translate declare_list_in_scope_exec'_def;
+
+val _ = translate AUPDATE_LIST_def;
+val _ = translate var_star_updates_of_func_map_def;
+val _ = translate var_star_updates_of_ext_map_def;
+val _ = translate initialise_var_stars_def;
+
+val _ = translate state_fin_exec_def;
+val _ = translate set_fin_status_def;
+
+(* 90s - uninit precondition (cheated on level below) *)
+val _ = translate arch_exec_def;
+
+val _ = translate arch_multi_exec_def;
+
+(******************************)
+(** Core arch implementation **)
+
+val _ = translate header_is_valid_def;
+
+val _ = translate header_set_valid_def;
+
+val _ = translate header_set_invalid_def;
+
+(* Common extern functions: *)
+val _ = translate oTAKE_DROP_def;
+val _ = translate v2w16s'''_def;
+val _ = translate header_entries2v_def;
+val _ = translate v2w16s''_def;
+val _ = translate get_checksum_incr''_def;
+
+val _ = translate add_with_carry'_def;
+val _ = translate add_ones_complement'_def;
+val _ = translate compute_checksum16_inner_def;
+val _ = translate all_lists_length_16_def;
+val _ = translate compute_checksum16_def;
+Theorem compute_checksum16_side:
+!v1. compute_checksum16_side v1
+Proof
+simp[Once $ definition "compute_checksum16_side_def"] \\
+Induct >- (
+ simp[Once $ theorem "compute_checksum16_inner_side_def", all_lists_length_16_def]
+) \\
+rpt strip_tac \\
+gs[all_lists_length_16_def, Once $ theorem "compute_checksum16_inner_side_def"] \\
+Cases_on ‘v1’ >- (
+ gs[theorem "compute_checksum16_inner_side_def",
+    compute_checksum16_inner_def, Once $ definition "add_ones_complement'_side_def",
+    Once $ definition "add_with_carry'_side_def"] \\
+ rpt strip_tac \\ (
+  gs[bitstringTheory.fixwidth_def, AllCaseEqs(), bitstringTheory.zero_extend_def,
+     listTheory.PAD_LEFT]
+ ) 
+) \\
+qpat_x_assum ‘!x2 x1. _’ (fn thm => ASSUME_TAC $ Q.SPECL [‘h'’, ‘t’] thm) \\
+simp[Once $ theorem "compute_checksum16_inner_side_def",
+     Once $ definition "add_ones_complement'_side_def",
+     Once $ definition "add_with_carry'_side_def"] \\
+rpt strip_tac >- (
+ gs[]
+) >- (
+ gs[compute_checksum16_inner_def, add_ones_complement'_def, add_with_carry'_def,
+    AllCaseEqs(), bitstringTheory.fixwidth_def, AllCaseEqs(),
+    bitstringTheory.zero_extend_def, listTheory.PAD_LEFT]
+) >- (
+ gs[]
+) >- (
+ gs[bitstringTheory.fixwidth_def, AllCaseEqs(), bitstringTheory.zero_extend_def,
+    listTheory.PAD_LEFT]
+) \\
+simp[Once $ theorem "compute_checksum16_inner_side_def"]
+QED
+val _ = update_precondition compute_checksum16_side;
+
+(* Shared over all architectures, so goes here *)
+val _ = translate p4_append_input_list_def;
+val _ = translate p4_get_output_list_def;
+val _ = translate word_def;
+
+val _ = ml_prog_update (close_module NONE);
+
+val _ = export_theory ();
