hol/symb_exec/tests/conditionalScript.sml
@@ -1,10 +1,10 @@
 open HolKernel boolLib liteLib simpLib Parse bossLib;
 
+val _ = new_theory "conditional";
+
 open p4Theory;
 
 open p4_symb_execLib;
-
-val _ = new_theory "conditional";
 
 (* Test 1:
  * There's a single if-statement that branches on symbolic bits.
@@ -154,6 +154,7 @@ val postcond_rewr_thms = [p4_symb_execTheory.packet_has_port_def]
 val postcond_simpset = pure_ss
 
 (* For debugging:
+val debug_flag = true;
 val comp_thm = INST_TYPE [Type.alpha |-> arch_ty] p4_exec_semTheory.arch_multi_exec_comp_n_tl_assl
 
 val fuel = 2
@@ -162,7 +163,7 @@ val ctx_name = "ctx"
 val ctx_def = hd $ Defn.eqns_of $ Defn.mk_defn ctx_name (mk_eq(mk_var(ctx_name, type_of ctx), ctx))
 
 val (path_tree, [(path_id, path_cond, step_thm)]) =
- p4_symb_exec 1 true arch_ty (ctx_def, ctx) (fty_map, b_fty_map, pblock_action_names_map) const_actions_tables init_astate stop_consts_rewr stop_consts_never [] path_cond NONE 1;
+ p4_symb_exec 1 true arch_ty (ctx_def, ctx) (fty_map, b_fty_map, pblock_action_names_map) const_actions_tables path_cond_defs init_astate stop_consts_rewr stop_consts_never [] path_cond NONE 3;
 *)
 
 
